examples/memcpy.v
@@ -1,0 +1,116 @@
+Require Import isla.base.
+Require Import isla.opsem.
+Require Import isla.automation.
+Require Import isla.adequacy.
+Require Import isla.examples.sys_regs.
+From isla.instructions Require Import a38236804 a38636824 a54ffff81 a91000463 ab40000e2 ad2800003 ad65f03c0 aeb03005f.
+
+
+(*
+C code:
+    void mcpy(unsigned char *dest, unsigned char *src, size_t n) {
+      for(size_t i = 0; i < n; i++ ) {
+        dest[i] = src[i];
+      }
+    }
+
+ASM:
+0000000000000000 <mcpy>:
+   0:	b40000e2 	cbz	x2, 1c <mcpy+0x1c>
+   4:	d2800003 	mov	x3, #0x0                   	// #0
+   8:	38636824 	ldrb	w4, [x1, x3]
+   c:	38236804 	strb	w4, [x0, x3]
+  10:	91000463 	add	x3, x3, #0x1
+  14:	eb03005f 	cmp	x2, x3
+  18:	54ffff81 	b.ne	8 <mcpy+0x8>  // b.any
+  1c:	d65f03c0 	ret
+*)
+
+Definition memcpy_loop_spec `{!islaG Σ} `{!threadG} : iProp Σ :=
+  ∃ (tmp src dst i n : bv 64) (srcdata dstdata : list byte) (pstaten pstatez pstatec pstatev : bv 1),
+  reg_col sys_regs ∗
+  "PSTATE" # "N" ↦ᵣ Val_Bits pstaten ∗ "PSTATE" # "Z" ↦ᵣ Val_Bits pstatez ∗
+  "PSTATE" # "C" ↦ᵣ Val_Bits pstatec ∗ "PSTATE" # "V" ↦ᵣ Val_Bits pstatev ∗
+  "R0" ↦ᵣ Val_Bits dst ∗ "R1" ↦ᵣ Val_Bits src ∗ "R2" ↦ᵣ Val_Bits n ∗
+  "R3" ↦ᵣ Val_Bits i ∗ "R4" ↦ᵣ Val_Bits tmp ∗
+  src ↦ₘ∗ srcdata ∗ dst ↦ₘ∗ dstdata ∗
+  ⌜bv_unsigned n = length srcdata⌝ ∗ ⌜bv_unsigned n = length dstdata⌝ ∗
+  ⌜bv_unsigned i < bv_unsigned n⌝ ∗
+  ⌜bv_unsigned src + bv_unsigned n < 2 ^ 52⌝ ∗
+  ⌜bv_unsigned dst + bv_unsigned n < 2 ^ 52⌝ ∗
+  ⌜take (Z.to_nat (bv_unsigned i)) dstdata = take (Z.to_nat (bv_unsigned i)) srcdata⌝ ∗
+  instr_pre 0x000000001030001c (
+    ∃ (tmp n : bv 64) (pstaten pstatez pstatec pstatev : bv 1),
+      reg_col sys_regs ∗
+      "PSTATE" # "N" ↦ᵣ Val_Bits pstaten ∗ "PSTATE" # "Z" ↦ᵣ Val_Bits pstatez ∗
+      "PSTATE" # "C" ↦ᵣ Val_Bits pstatec ∗ "PSTATE" # "V" ↦ᵣ Val_Bits pstatev ∗
+      "R0" ↦ᵣ Val_Bits dst ∗ "R1" ↦ᵣ Val_Bits src ∗ "R2" ↦ᵣ Val_Bits n ∗
+      "R4" ↦ᵣ Val_Bits tmp ∗ "R3" ↦ᵣ Val_Bits n ∗
+      src ↦ₘ∗ srcdata ∗ dst ↦ₘ∗ srcdata ∗
+      True
+  )
+.
+
+Arguments memcpy_loop_spec /.
+
+Lemma memcpy_loop `{!islaG Σ} `{!threadG} :
+  instr 0x0000000010300008 (Some a38636824) -∗
+  instr 0x000000001030000c (Some a38236804) -∗
+  instr 0x0000000010300010 (Some a91000463) -∗
+  instr 0x0000000010300014 (Some aeb03005f) -∗
+  instr 0x0000000010300018 (Some a54ffff81) -∗
+  □ instr_pre 0x0000000010300008 memcpy_loop_spec -∗
+  instr_body 0x0000000010300008 memcpy_loop_spec.
+Proof.
+  iStartProof.
+  Time repeat liAStep; liShow.
+  liInst Hevar (Z.to_nat (bv_unsigned i)).
+  Time repeat liAStep; liShow.
+  liInst Hevar (Z.to_nat (bv_unsigned i)).
+  Time repeat liAStep; liShow.
+
+  Unshelve. all: prepare_sidecond.
+  all: try bv_solve.
+  - rename select (bv_extract _ _ _ ≠ _) into Hextract.
+    (* TODO: use some lemma to turn bv_not into bv_opp / bv_sub *)
+    admit.
+  - admit.
+  - admit.
+  - admit.
+Abort.
+
+Lemma memcpy `{!islaG Σ} `{!threadG} :
+  instr 0x0000000010300000 (Some ab40000e2) -∗
+  instr 0x0000000010300004 (Some ad2800003) -∗
+  instr 0x000000001030001c (Some ad65f03c0) -∗
+  □ instr_pre 0x0000000010300008 memcpy_loop_spec -∗
+  instr_body 0x0000000010300000 (
+    ∃ (tmp1 tmp2 src dst n ret : bv 64) (srcdata dstdata : list byte) (pstaten pstatez pstatec pstatev : bv 1),
+    reg_col sys_regs ∗
+    "PSTATE" # "N" ↦ᵣ Val_Bits pstaten ∗ "PSTATE" # "Z" ↦ᵣ Val_Bits pstatez ∗
+    "PSTATE" # "C" ↦ᵣ Val_Bits pstatec ∗ "PSTATE" # "V" ↦ᵣ Val_Bits pstatev ∗
+    "R0" ↦ᵣ Val_Bits dst ∗ "R1" ↦ᵣ Val_Bits src ∗ "R2" ↦ᵣ Val_Bits n ∗
+    "R3" ↦ᵣ Val_Bits tmp2 ∗ "R4" ↦ᵣ Val_Bits tmp1 ∗
+    "R30" ↦ᵣ Val_Bits ret ∗
+    src ↦ₘ∗ srcdata ∗ dst ↦ₘ∗ dstdata ∗
+    ⌜bv_unsigned n = length srcdata⌝ ∗ ⌜bv_unsigned n = length dstdata⌝ ∗
+    ⌜bv_unsigned src + bv_unsigned n < 2 ^ 52⌝ ∗
+    ⌜bv_unsigned dst + bv_unsigned n < 2 ^ 52⌝ ∗
+    instr_pre (bv_unsigned ret) (
+    ∃ (tmp1 tmp2 n : bv 64) (pstaten pstatez pstatec pstatev : bv 1),
+      reg_col sys_regs ∗
+      "PSTATE" # "N" ↦ᵣ Val_Bits pstaten ∗ "PSTATE" # "Z" ↦ᵣ Val_Bits pstatez ∗
+      "PSTATE" # "C" ↦ᵣ Val_Bits pstatec ∗ "PSTATE" # "V" ↦ᵣ Val_Bits pstatev ∗
+      "R0" ↦ᵣ Val_Bits dst ∗ "R1" ↦ᵣ Val_Bits src ∗ "R2" ↦ᵣ Val_Bits n ∗
+      "R3" ↦ᵣ Val_Bits tmp2 ∗ "R4" ↦ᵣ Val_Bits tmp1 ∗
+      "R30" ↦ᵣ Val_Bits ret ∗
+      src ↦ₘ∗ srcdata ∗ dst ↦ₘ∗ srcdata ∗
+      True
+  )).
+Proof.
+  iStartProof.
+  Time repeat liAStep; liShow.
+  Unshelve. all: prepare_sidecond.
+  - by destruct dstdata, srcdata.
+  - bv_simplify_hyp select (n ≠ _). bv_solve.
+Time Qed.
